Outcome.v
@@ -9,14 +9,9 @@ Local Open Scope core_scope.
 Local Open Scope nat_scope.
 Local Open Scope list_scope.
 
-Module Values.
-  Definition t := Z.
-End Values.
-Module Store := MakeStore (Values).
-Import Store.
-
 Section Outcome.
 
+Definition store := store Z.
 Definition measure := store -> nat.
 Definition measure_lex (s:store) (a b:measure) : Prop := a s < b s.
 Definition measure_le (a b:measure) : Prop :=
